core/Net.v
@@ -35,17 +35,17 @@ Class MultiParams (P : BaseParams) :=
     input_handlers : name -> input -> data -> (list output) * data * list (name * msg)
   }.
 
+Class FailureParams `(P : MultiParams) :=
+  {
+    reboot : data -> data
+  }.
+
 Class NameOverlayParams `(P : MultiParams) :=
   {
     adjacent_to : relation name;
     adjacent_to_dec : forall x y : name, {adjacent_to x y} + {~ adjacent_to x y};
     adjacent_to_symmetric : Symmetric adjacent_to;
     adjacent_to_irreflexive : Irreflexive adjacent_to
-  }.
-
-Class FailureParams `(P : MultiParams) :=
-  {
-    reboot : data -> data
   }.
 
 Class FailMsgParams `(P : MultiParams) :=
@@ -57,6 +57,49 @@ Class NewMsgParams `(P : MultiParams) :=
   {
     msg_new : msg
   }.
+
+Class EqDec_eq (A : Type) := eq_dec : forall (x y : A), {x = y} + {x <> y}.
+
+Class RelDec {A : Type} (R : relation A) := rel_dec : forall (x y : A), {R x y} + {~ R x y}.
+
+Instance EqDec_eq_name `{params : MultiParams} : EqDec_eq name := name_eq_dec.
+
+Instance EqDec_eq_msg `{params : MultiParams} : EqDec_eq msg := msg_eq_dec.
+
+Instance RelDec_adjacent_to `{params : NameOverlayParams} : RelDec adjacent_to := adjacent_to_dec.
+
+Section DecDefs.
+  Context {A : Type}.
+  Context {ea : EqDec_eq A}.
+  Context {R : relation A} {rd : RelDec R}.
+
+  Definition update' {B} st h (v : B) := fun nm => if eq_dec nm h then v else st nm.
+
+  Definition update2 {B} (f : A -> A -> B) (x y : A) (v : B) : A -> A -> B :=
+    fun x' y' => if sumbool_and _ _ _ _ (eq_dec x x') (eq_dec y y')
+                then v
+                else f x' y'.
+
+  Definition update_opt {B} st h (v : B) := fun nm => if eq_dec nm h then Some v else st nm.
+
+  Fixpoint collate {B} (from : A) (f : A -> A -> list B) (ms : list (A * B)) : A -> A -> list B :=
+    match ms with
+    | [] => f
+    | (to, m) :: ms' => collate from (update2 f from to (f from to ++ [m])) ms'
+    end.
+
+  Fixpoint collate_ls {B} (s : list A) (f : A -> A -> list B) (to : A) (m : B) : A -> A -> list B :=
+    match s with
+    | [] => f
+    | from :: s' => collate_ls s' (update2 f from to (f from to ++ [m])) to m
+    end.
+
+  Definition exclude (excluded : list A) := filter (fun a => if (in_dec eq_dec a excluded) then false else true).
+  
+  Definition map_pair {B} (b : B) := map (fun (a : A) => (a, b)).
+  
+  Definition filter_rel (a : A) := filter (fun a' => if rel_dec a a' then true else false).
+End DecDefs.
 
 Section StepRelations.
   Variable A : Type.
@@ -422,28 +465,17 @@ Section StepOrder.
          onwState   : name -> data
        }.
 
-  Definition update2 {A} (f : name -> name -> A) (x y : name) (v : A) : name -> name -> A :=
-    fun x' y' => if sumbool_and _ _ _ _ (name_eq_dec x x') (name_eq_dec y y')
-              then v
-              else f x' y'.
-
-  Fixpoint collate (from : name) (f : name -> name -> list msg) (ms : list (name * msg)) : name -> name -> list msg :=
-    match ms with
-    | [] => f
-    | (to, m) :: ms' => collate from (update2 f from to (f from to ++ [m])) ms'
-    end.
-
   Inductive step_o : step_relation ordered_network (name * (input + list output)) :=
   | SO_deliver : forall net net' m ms out d l from to,
                      onwPackets net from to = m :: ms ->
                      net_handlers to from m (onwState net to) = (out, d, l) ->
                      net' = mkONetwork (collate to (update2 (onwPackets net) from to ms) l)
-                                      (update (onwState net) to d) ->
+                                      (update' (onwState net) to d) ->
                      step_o net net' [(to, inr out)]
   | SO_input : forall h net net' out inp d l,
                    input_handlers h inp (onwState net h) = (out, d, l) ->
                    net' = mkONetwork (collate h (onwPackets net) l)
-                                     (update (onwState net) h d) ->
+                                     (update' (onwState net) h d) ->
                    step_o net net' [(h, inl inp); (h, inr out)].
 
   Definition step_o_star := refl_trans_1n_trace step_o.
@@ -457,29 +489,23 @@ Section StepOrderFailure.
   Context {overlay_params : NameOverlayParams multi_params}.
   Context {fail_msg_params : FailMsgParams multi_params}.
 
-  Definition msg_for (m : msg) := map (fun (n : name) => (n, m)).
-
-  Definition exclude (excluded : list name) := filter (fun n => if (in_dec name_eq_dec n excluded) then false else true).
-
-  Definition adjacent_to_node (n : name) := filter (fun n' => if adjacent_to_dec n n' then true else false).
-
   Inductive step_o_f : step_relation (list name * ordered_network) (name * (input + list output)) :=
   | SOF_deliver : forall net net' failed m ms out d l from to,
                      onwPackets net from to = m :: ms ->
                      ~ In to failed ->
                      net_handlers to from m (onwState net to) = (out, d, l) ->
                      net' = {| onwPackets := collate to (update2 (onwPackets net) from to ms) l;
-                               onwState := update (onwState net) to d |} ->
+                               onwState := update' (onwState net) to d |} ->
                      step_o_f (failed, net) (failed, net') [(to, inr out)]
   | SOF_input : forall h net net' failed out inp d l,
                    ~ In h failed ->
                    input_handlers h inp (onwState net h) = (out, d, l) ->
                    net' = {| onwPackets := collate h (onwPackets net) l;
-                             onwState := update (onwState net) h d |} ->
+                             onwState := update' (onwState net) h d |} ->
                    step_o_f (failed, net) (failed, net') [(h, inl inp); (h, inr out)]
   | SOF_fail :  forall h net net' failed,
                  ~ In h failed ->
-                 net' = {| onwPackets := collate h (onwPackets net) (msg_for msg_fail (adjacent_to_node h (exclude failed nodes)));
+                 net' = {| onwPackets := collate h (onwPackets net) (map_pair msg_fail (filter_rel h (exclude failed nodes)));
                            onwState := onwState net |} ->
                  step_o_f (failed, net) (h :: failed, net') [].
 
@@ -494,8 +520,6 @@ Section StepOrderDynamic.
   Context {overlay_params : NameOverlayParams multi_params}.
   Context {new_msg_params : NewMsgParams multi_params}.
 
-  Definition update_opt {A : Type} st h (v : A) := fun nm => if name_eq_dec nm h then Some v else st nm.
-
   Notation src := name (only parsing).
   Notation dst := name (only parsing).
 
@@ -507,19 +531,12 @@ Section StepOrderDynamic.
          odnwState : name -> option data
        }.
 
-  Fixpoint collate_ls (s : list name) (f : name -> name -> list msg) (to : name) (m : msg) : name -> name -> list msg :=
-  match s with
-  | [] => f
-  | from :: s' =>
-    collate_ls s' (update2 f from to (f from to ++ [m])) to m
-  end.
-
   Inductive step_o_d : step_relation ordered_dynamic_network (name * (input + list output)) :=
   | SOD_start : forall net net' h,
       ~ In h (odnwNodes net) ->
       net' = {| odnwNodes := h :: odnwNodes net;
-                odnwPackets := collate_ls (adjacent_to_node h (odnwNodes net))
-                               (collate h (odnwPackets net) (msg_for msg_new (adjacent_to_node h (odnwNodes net))))
+                odnwPackets := collate_ls (filter_rel h (odnwNodes net))
+                               (collate h (odnwPackets net) (map_pair msg_new (filter_rel h (odnwNodes net))))
                                h msg_new;
                 odnwState := update_opt (odnwState net) h (init_handlers h) |} ->
       step_o_d net net' []
@@ -557,8 +574,8 @@ Section StepOrderDynamicFailure.
   | SODF_start : forall net net' failed h,
       ~ In h (odnwNodes net) ->
       net' = {| odnwNodes := h :: odnwNodes net;
-                odnwPackets := collate_ls (adjacent_to_node h (exclude failed (odnwNodes net)))
-                               (collate h (odnwPackets net) (msg_for msg_new (adjacent_to_node h (exclude failed (odnwNodes net)))))
+                odnwPackets := collate_ls (filter_rel h (exclude failed (odnwNodes net)))
+                               (collate h (odnwPackets net) (map_pair msg_new (filter_rel h (exclude failed (odnwNodes net)))))
                                h msg_new;
                 odnwState := update_opt (odnwState net) h (init_handlers h) |} ->
       step_o_d_f (failed, net) (failed, net') []
@@ -585,7 +602,7 @@ Section StepOrderDynamicFailure.
       ~ In h failed ->
       In h (odnwNodes net) ->
       net' = {| odnwNodes := odnwNodes net;
-                odnwPackets := collate h (odnwPackets net) (msg_for msg_fail (adjacent_to_node h (exclude failed (odnwNodes net))));
+                odnwPackets := collate h (odnwPackets net) (map_pair msg_fail (filter_rel h (exclude failed (odnwNodes net))));
                 odnwState := odnwState net |} ->
       step_o_d_f (failed, net) (h :: failed, net') [].
 
